\documentclass[thesis.tex]{subfiles}

\begin{document}

\iffulldocument\else
	\chapter{KdV5}
\fi

\section{Inversion}

We will now solve the system \cref{eigsystem}. The proof follows the outline of \cite[Theorem 2]{Sandstede1998}, with the main differences being the presence of a center subspace and the fact that we are on a periodic domain. Define the spaces
\begin{align*}
V_a &= \bigoplus_{i=0}^{n-1} E^u(0) \oplus E^s(0) \oplus E^c(0) \\
V_b &= \bigoplus_{i=0}^{n-1} E^u(0) \oplus E^s(0) \\
V_c &= \bigoplus_{i=0}^{n-1} \C \\
V_d &= \bigoplus_{i=0}^{n-1} \C \\
V_\lambda &= B_\delta(0) \subset \C
\end{align*}
where the subscripts are all taken $\Mod n$, since we are on a periodic domain. All the product spaces are endowed with the maximum norm, e.g. for $V_b$, 
\[
|b| = \max(|b_0^-|, \dots, |b_{n-1}^-|, |b_0^+|, \dots, |b_{n-1}^+|)
\]

As in \cite{Sandstede1998}, we will write \eqref{systemZ} in integrated form as a set of fixed point equations. Using the variation of constants formula and splitting the evolution using the exponential trichotomy from \cref{sec:trichotomy}, we write \eqref{systemZ} as the set of fixed point equations
\begin{equation}\label{Zfpeq}
\begin{aligned}
Z&_i^-(x) = \Phi^s_{i,-}(x, -X_{i-1}; \lambda) P^i_-(-X_{i-1}, \lambda)^{-1} a_{i-1}^- + \Phi^u_-(x, 0; \lambda) b_i^- - \Phi^c_{i,-}(x, -X_{i-1}; \lambda) P^i_-(-X_{i-1}, \lambda)^{-1} a_{i-1}^c \\
&+ \int_0^x \Phi^u_-(x, y; \lambda)P^i_-(y; \lambda)^{-1} [ c_{i-1} e^{\nu(\lambda)X_{i-1}} G_i^-(y) V^-(y; \lambda) + \lambda^2 d_i \tilde{H}_i^-(y)] dy \\
&+ \int_{-X_{i-1}}^x \Phi^s_{i,-}(x, y; \lambda) P^i_-(y; \lambda)^{-1}[ c_{i-1} e^{\nu(\lambda)X_{i-1}} G_i^-(y) V^-(y; \lambda) + \lambda^2 d_i \tilde{H}_i^-(y)] dy \\
&+ \int_{-X_{i-1}}^x \Phi^c_{i,-}(x, y; \lambda) P^i_-(y; \lambda)^{-1}[ c_{i-1} e^{\nu(\lambda)X_{i-1}} G_i^-(y) V^-(y; \lambda) + \lambda^2 d_i \tilde{H}_i^-(y)] dy  \\ 
Z&_i^+(x) = \Phi^u_{i,+}(x, X_i; \lambda) P^i_+(X_i, \lambda)^{-1} a_i^+ + \Phi^s_+(x, 0; \lambda) b_i^+ + \Phi^c_{i,+}(x, X_i; \lambda) P^i_+(X_i, \lambda)^{-1} a_i^c \\
&+ \int_0^x \Phi^s_+(x, y; \lambda) P^i_+(y; \lambda)^{-1} [ c_i e^{-\nu(\lambda)X_i} G_i^-(y)V^+(y; \lambda) + \lambda^2 d_i \tilde{H}_i^+(y)] dy \\
&+ \int_{X_i}^x \Phi^u_{i,+}(x, y; \lambda) P^i_+(y; \lambda)^{-1} [ c_i e^{-\nu(\lambda)X_i} G_i^-(y)V^+(y; \lambda) + \lambda^2 d_i \tilde{H}_i^+(y)] dy \\
&+ \int_{X_i}^x \Phi^c_{i,+}(x, y; \lambda) P^i_+(y; \lambda)^{-1} [ c_i e^{-\nu(\lambda)X_i} G_i^-(y)V^+(y; \lambda) + \lambda^2 d_i \tilde{H}_i^+(y)] dy \\
\end{aligned}
\end{equation}
As in \cite{Sandstede1998}, we will solve the eigenvalue problem in a series of inversion steps. Since the RHS of the fixed point equations \cref{Zfpeq} does not involve $Z_i^\pm$, these equations give the solution for \cref{systemZ}. In the first lemma, we solve \cref{systemmiddle}, which are the matching conditions at the tails.

% first inversion lemma : match at \pm X_i
\begin{lemma}\label{Zinv1}
There exists an operator
\begin{align*}
A_1: V_\lambda \times V_b \times V_c \times V_d \rightarrow V_a \\
\end{align*}
such that 
\[
a = A_1(\lambda)(b, c, d)
\]
solves \eqref{systemmiddle} for any $(b, c, d)$ and $\lambda$. This operator is analytic in $\lambda$ and linear in $(b, c, d)$. Bounds for $A_1$ are given by
\begin{align}\label{A1bound}
|A_1(\lambda)(b, c, d)| \leq C \left( e^{-\alpha X^*} |b| + (e^{-\alpha X^*} + |C_i|)|c| + |\lambda|^2 |d| + |D_i||d| \right)
\end{align} 

\begin{proof}
At $\pm X_i$, the fixed point equations \eqref{Zfpeq} are
\begin{align*}
Z_{i+1}^-&(-X_i) = \Phi^s_{i+1,-}(-X_i, -X_i; \lambda) P^{i+1}_-(-X_i, \lambda)^{-1} a_{i-1}^-  - \Phi^c_{i+1,-}(-X_i, -X_i; \lambda) P^{i+1}_-(-X_i, \lambda)^{-1} a_i^c \\ 
&+ \Phi^u_-(-X_i, 0; \lambda) b_{i+1}^-
+ \int_0^{-X_i} \Phi^u_-(-X_i, y; \lambda) P^{i+1}_-(y; \lambda)^{-1} \big[ c_i e^{\nu(\lambda)X_i} G_{i+1}^-(y) V^-(x; \lambda) + \lambda^2 d_{i+1} \tilde{H}_{i+1}^-(y)\big] dy \\
Z_i^+&(X_i) = \Phi^u_{i,+}(X_i, X_i; \lambda) P^i_+(X_i, \lambda)^{-1} a_i^+ + \Phi^c_{i,+}(X_i, X_i; \lambda) P^i_+(X_i, \lambda)^{-1} a_i^c \\
&+ \Phi^s_+(X_i, 0; \lambda) b_i^+ 
+ \int_0^{X_i} \Phi^s_+(X_i, y; \lambda) P^i_+(y; \lambda)^{-1} \big[ c_i e^{-\nu(\lambda)X_i} G_i^-(y) V^+(y; \lambda) + \lambda^2 d_i \tilde{H}_i^+(y)\big] dy
\end{align*}
Applying the appropriate conjugation operators and subtracting, we obtain the equation 
\begin{equation}\label{Dideq0}
\begin{aligned}
D_i &d + C_i c = P^i_+(X_i, \lambda) \Phi^u_{i,+}(X_i, X_i; \lambda) P^i_+(X_i, \lambda)^{-1} a_i^+ +  P^i_+(X_i, \lambda) \Phi^c_{i,+}(X_i, X_i; \lambda) P^i_+(X_i, \lambda)^{-1} a_i^c \\
&+ P^i_+(X_i; \lambda)\Phi^s_+(X_i, 0; \lambda) b_i^+ \\
&+ P^i_+(X_i; \lambda) \int_0^{X_i} \Phi^s_+(X_i, y; \lambda) P^i_+(y; \lambda)^{-1}\big[ c_i e^{-\nu(\lambda)X_i} G_i^-(y) V^+(y; \lambda) + \lambda^2 d_i \tilde{H}_i^+(y) \big] dy \\
&- P^{i+1}_-(-X_i, \lambda) \Phi^s_{i+1,-}(-X_i,-X_i; \lambda) P^{i+1}_-(-X_i, \lambda)^{-1} a_i^- + P^{i+1}_-(-X_i, \lambda) \Phi^c_{i+1,-}(-X_i,-X_i; \lambda) P^{i+1}_-(-X_i, \lambda)^{-1} a_i^c  \\ 
&- P^{i+1}_-(-X_i; \lambda)\Phi^u(-X_i, 0; \lambda) b_{i+1}^- \\
&- P^{i+1}_-(-X_i; \lambda) \int_0^{-X_i} \Phi^u_-(-X_i, y; \lambda) P^{i+1}_-(y; \lambda)^{-1}\big[ c_i e^{\nu(\lambda)X_i} G_{i+1}^-(y) V^-(y; \lambda) + \lambda^2 d_{i+1} \tilde{H}_{i+1}^-(y)\big] dy.
\end{aligned}
\end{equation}
From \cref{sec:trichotomy}, 
\begin{align*}
P^{i+1}_-(-X_i, \lambda) \Phi^{s/c}_{i+1,-}(-X_i, -X_i; \lambda) P^{i+1}_-(-X_i, \lambda)^{-1} &= \tilde{\Phi}^{s/c}_{i+1,-}(-X_i, -X_i; \lambda) = P^{s/c}(0) \\
P^i_+(X_i, \lambda) \Phi^{u/c}_{i,+}(X_i, X_i; \lambda) P_+(X_i, \lambda)^{-1} &= \tilde{\Phi}^{u/c}_{i,+}(X_i, X_i; \lambda) = P^{u/c}(0),
\end{align*}
thus we have
\begin{equation}\label{Didexpansion}
\begin{aligned}
D_i &d + C_i c = a_i^+ - a_i^- + 2 a_i^c \\
&+ P^i_+(X_i; \lambda)\Phi^s_+(X_i, 0; \lambda) b_i^+ - P^{i+1}_-(-X_i; \lambda)\Phi^u_-(-X_i, 0; \lambda) b_{i+1}^- \\
&+ P^i_+(X_i; \lambda) \int_0^{X_i} \Phi^s_+(X_i, y; \lambda) P^i_+(y; \lambda)^{-1}\big[ c_i e^{-\nu(\lambda)X_i} G_i^-(y) V^+(y; \lambda) + \lambda^2 d_i \tilde{H}_i^+(y)\big] dy \\ 
&- P^{i+1}_-(-X_i; \lambda) \int_0^{-X_i} \Phi^u(-X_i, y; \lambda) P^{i+1}_-(y; \lambda)^{-1}\big[ c_i e^{\nu(\lambda)X_i} G_{i+1}^-(y) V^-(y; \lambda) + \lambda^2 d_{i+1} \tilde{H}_{i+1}^-(y)\big] dy
\end{aligned}
\end{equation}
This is of the form
\begin{align}\label{Dideq1}
D_i d + C_i c &= a_i^+ - a_i^- + 2 a_i^c + L_3(\lambda)_i(b, c, d)
\end{align}
where the linear operator $L_3(\lambda)_i(b, c, d)$ is defined by the RHS of \cref{Didexpansion} (note that there is no dependence on $a$). $L_3(\lambda)_i(b, c, d)$ is linear in $(a,b,c,d)$ and analytic in $\lambda$. To get a bound on $L_3$, we will bound the individual terms. 
\begin{enumerate}
\item For the terms involving $b$, we use the exponential dichotomy bounds \eqref{Zevolbounds} to get
\[
| P_+(X_i; \lambda)\Phi^s(X_i, 0; \lambda) b_i^+ - P_-(-X_i; \lambda) \Phi^u(-X_i, 0; \lambda) b_{i+1}^-| \leq C e^{-\alpha X^*} |b|
\]
\item For the integral terms involving $\tilde{H}_i^\pm$, by \eqref{Zevolbounds} and the estimates from Lemma \ref{stabestimateslemma}, we have
\begin{align*}
&\left|
P^{i+1}_-(-X_i; \lambda) \int_0^{-X_i} \Phi^u_-(-X_i, y; \lambda) P^{i+1}_-(y; \lambda)^{-1} \lambda^2 d_{i+1} \tilde{H}_{i+1}^-(y) dy \right| \\
& \leq C |\lambda|^2 |d| \int_{-X_i}^0 e^{-\alpha(X_i + y)} e^{\alpha y} dy \\
& \leq C |\lambda|^2 |d|
\end{align*}
The other integral is similar.

\item For the integral terms involving $G_i^\pm(x)$, we have by \eqref{Zevolbounds}, \cref{lemma:expnubound}, and the estimates from \cref{stabestimateslemma},
\begin{align*}
&\left|
P^{i+1}_-(-X_i; \lambda) \int_0^{-X_i} \Phi^u_-(-X_i, y; \lambda) P^{i+1}_-(y; \lambda)^{-1} c_i e^{\nu(\lambda)X_i} G_{i+1}^-(y) V^-(y; \lambda) dy \right| \\
&\leq C |c| \int_0^{-X_i} e^{-\alpha(X_i + y)} \left( e^{-\alpha X_i} e^{-\alpha(X_i + y) } + e^{-2 \alpha X_i} e^{\alpha y} \right) dy \\
&\leq C e^{-\alpha X^*} |c| 
\end{align*}
The other integral is similar.
\end{enumerate}

Putting all of these together, we have the bound for $L_3$.
\begin{equation}\label{L3bound}
|L_3(\lambda)(b, c, d)| \leq C \left( e^{-\alpha X^*} |b| + e^{-\alpha X^*} |c| + |\lambda|^2 |d| \right)
\end{equation}
Let 
\[
J_1: \bigoplus_{j=1}^n (E^s(\lambda) \times E^u(
\lambda) \times E^c(\lambda) ) \rightarrow \bigoplus_{j=1}^n \rightarrow \C^{2m+1}
\]
be defined by $(J_1)_i(a_i^+, a_i^-, 2 a_i^c V_0(\lambda)) = a_i^+ - a_i^- + 2 a_i^c$, which is a linear isomorphism since $E^s(0) \oplus E^u(0) \oplus E^c(0) = \C^{2m+1}$. Then from \cref{Dideq1}, we can solve for $a$ using  
\[
a = A_1(\lambda)(b, c, d) = J_1^{-1} \left(D_i d + C_i c - L_3(\lambda)(b, c, d)\right)
\]
Using the bounds on $L_3$, $A_1$ has bound given by \cref{A1bound}.
\end{proof}
\end{lemma}

Next, we derive expressions for $a_i^\pm$ and $a_i^c$ which we will use in evaluating the jump conditions.

\begin{lemma}\label{lemma:aipm}
For the initial conditions $a_i^\pm$ and $a_i^c$, we have the expressions
\begin{equation}\label{aipmexp1}
\begin{aligned}
a_i^+ &= P_0^u(\lambda) D_i d + A_2(\lambda)_i^+(b, c, d) \\
a_i^- &= -P_0^s(\lambda) D_i d + A_2(\lambda)_i^-(b, c, d) \\
a_i^c &= \tilde{A}_2(\lambda)_i(b, c, d).
\end{aligned}
\end{equation}
$A_2$ and $\tilde{A}^2$ are linear in $(b, c, d)$, and have bounds
\begin{align}
|A_2(\lambda)_i(b, c, d)|
&\leq C \left(e^{-\alpha X^*}|b| + e^{-\alpha X^*}|c| + |\lambda|^2|d| \right) \label{A2bound} \\
|\tilde{A}_2(\lambda)(b, c, d) &\leq C |\lambda| e^{-\alpha X_i} \left( e^{-\alpha X^*}  |b| + |c| +|\lambda|^2 |d| \right) \label{tildeA2bound}
\end{align}

\begin{proof}
First, we apply the projections $P^{s/u}(0)$ on the eigenspaces $E^{s/u}(0)$ to \eqref{Dideq1}. Using the bound $|C_i c| \leq e^{-\alpha X^*}|c|$ from Lemma \ref{stabestimateslemma} and the bound for $L_3$ from \cref{Zinv1}, we obtain the expressions
\begin{align*}
a_i^+ &= P_0^u(0) D_i d + A_2(\lambda)_i^+(b, c, d) \\
a_i^- &= -P_0^s(0) D_i d + A_2(\lambda)_i^-(b, c, d),
\end{align*}
where 
\begin{align*}
|A_2&(\lambda)_i(b, c, d)| \leq C \left(e^{-\alpha X^*}|b| + e^{-\alpha X^*}|c| + |\lambda|^2|d| \right)
\end{align*} 
For $a_i^c$, we apply the center projection $P^c(0) = \langle W_0, \cdot \rangle$ to \eqref{Dideq1}. $\langle W_0, D_i d\rangle = 0$, and for $P^c(0) C_i c$, we write $C_i c$ as 
\begin{align*}
C_i c &= c_i \left( e^{\nu(\lambda) X_i} V^-(-X_i; \lambda) - e^{-\nu(\lambda) X_i} V^+(X_i; \lambda) \right) \\
&= c_i \left( e^{\nu(\lambda) X_i} e^{\nu(\lambda)X_i} P_-(-X_i; \lambda) V_0(\lambda) - e^{-\nu(\lambda) X_i} e^{\nu(\lambda)X_i} P_+(X_i; \lambda)V_0(\lambda) \right) \\
&= c_i \left( P_-(-X_i; \lambda) - P_+(X_i; \lambda) \right) V_0(\lambda) \\
&= c_i \left( R \Theta_+(X_i; \lambda) R - \Theta_+(X_i; \lambda) \right) V_0(\lambda),
\end{align*}
where in the last line we used \cref{defPminus} and the expansion \cref{conjlemmaP} for the conjugation operator. Expanding $\Theta_+(X_i; \lambda)$ and $V_0(\lambda)$ in a Taylor series about $\lambda = 0$, this becomes
\begin{align*}
C_i c &= c_i \left( R \Theta_+(X_i; 0) R - \Theta_+(X_i; 0) + \mathcal{O}(|\lambda|e^{-\alpha X_i}) \right) (V_0 + \mathcal{O}(|\lambda|)) \\
&= c_i \left( R \Theta_+(X_i; 0) R - \Theta_+(X_i; 0) \right) V_0 + \mathcal{O}(|\lambda|e^{-\alpha X_i}|c|)
\end{align*}
Taking the inner product with $W_0$, this becomes
\begin{align*}
\langle W_0, C_i c \rangle &=  c_i \langle W_0, \left( R \Theta_+(X_i; 0) R - \Theta_+(X_i; 0) \right) V_0 \rangle + \mathcal{O}(|\lambda|e^{-\alpha X_i}|c| ) \\
&= c_i \left( \langle R W_0, \Theta_+(X_i; 0) R V_0 \rangle - \langle W_0, \Theta_+(X_i; 0), V_0 \rangle \right) + \mathcal{O}(|\lambda|e^{-\alpha X_i}|c| ) \\
&= \mathcal{O}(|\lambda|e^{-\alpha X_i}|c| )
\end{align*}
since $R W_0 = W_0$ and $RV_0 = V_0$. Finally, we evaluate $P^c(0)L_3(\lambda)_i(b,c,d)$ by using \cref{W0projlemma}(iv) together with the bounds we obtained for the terms of $L_3(\lambda)_i(b,c,d)$ from \cref{Zinv1} to get 
\begin{equation*}
|P^c(\lambda)\tilde{L}_3(\lambda)_i(a,b,c,d)| \leq C |\lambda| e^{-\alpha X_i} \left( e^{-\alpha X^*} |b| + e^{-\alpha X^*} |c| + |\lambda|^2 |d| \right)
\end{equation*}
Combining everything and dividing by 2, we have 
\begin{equation*}
a_i^c = \tilde{A}_2(\lambda)(b, c, d),
\end{equation*}
where we have bound
\begin{align*}
|\tilde{A}_2(\lambda)(b, c, d) \leq C |\lambda| e^{-\alpha X_i} \left( e^{-\alpha X^*}  |b| + |c| +|\lambda|^2 |d| \right)
\end{align*}
\end{proof}
\end{lemma}

In the next lemma, we solve equations \cref{systemcenter1} and \cref{systemcenter1}, which are the non-jump matching conditions at $x = 0$.
\begin{equation}\label{centercond}
\begin{aligned}
P^i_\pm(0; \lambda) Z_i^\pm(0) &\in \oplus Y^+ \oplus Y^- \oplus \C \Psi(0) \oplus \C \Psi^c(0) \\
P^i_+(0; \lambda) Z_i^+(0) - P^i_-(0; \lambda) Z_i^-(0) &\in \C \Psi(0) \oplus \C \Psi^c(0)
\end{aligned}
\end{equation}
Recall that we have the decomposition
\begin{equation}\label{DSdecomp}
\C^{2m+1} = \C Q'(0) \oplus Y^+ \oplus Y^- \oplus \C \Psi(0) \oplus \C \Psi^c(0)
\end{equation}
Thus \eqref{centercond} is equivalent to the three projections
\begin{equation}\label{centercond2}
\begin{aligned}
P(\C Q'(0) ) P^i_-(0; \lambda) Z_i^-(0) &= 0 \\
P(\C Q'(0) ) P^i_+(0; \lambda) Z_i^+(0) &= 0 \\
P(Y_i^+ \oplus Y_i^-) ( P^i_+(0; \lambda) Z_i^+(0) - P^i_-(0; \lambda) Z_i^-(0) ) &= 0
\end{aligned}
\end{equation}
where the kernel of each projection is the remaining spaces in the direct sum decomposition \eqref{DSdecomp}. We do not need to include $\C Q'(0)$ in the third equation of \eqref{centercond2} since we eliminated any component in $\C Q'(0)$ in the first two equations.

% second inversion lemma
\begin{lemma}\label{Zinv2}
There exist operators
\begin{align*}
B_1: &V_\lambda \times V_c \times V_d \rightarrow V_b \\
A_3: &V_\lambda \times V_c \times V_d \rightarrow V_a \\
\end{align*}
such that $( a, b ) = ( A_3(\lambda)(c, d), B_1(\lambda)(c, d) )$ solves \eqref{systemmiddle}, \eqref{systemcenter1}, and \eqref{systemcenter2} for any $(c, d)$. These operators are analytic in $\lambda$ and linear in $(c, d)$. Bounds for $B_1$ and $A_3$ are given by
\begin{align}
|B_1(\lambda)(c, d)| &\leq C\Big( e^{-\alpha X^*}|c| + (|\lambda| + e^{-\alpha X^*})^2 |d| \Big) \label{B1bound} \\
|A_3(\lambda)(b, c, d)| &\leq C \left( e^{-\alpha X^*} |c| + |\lambda|^2 |d| + |D_i||d| \right) \label{A3bound} 
\end{align} 
In addition, we can write
\begin{align*}
a_i^+ &= P_0^u(0) D_i d + A_4(\lambda)_i^+(c, d) \\
a_i^- &= -P_0^s(0) D_i d + A_4(\lambda)_i^-(c, d) \\
a_i^c &= \tilde{A}_4(\lambda)_i(c, d) 
\end{align*}
where $A_4$ and $\tilde{A}_4$ are linear in $(c, d)$, and have bounds
\begin{align}
|A_4(\lambda)(b, c, d)|
&\leq C \left( e^{-\alpha X^*}|c| + (|\lambda| + e^{-\alpha X^*})^2 |d| ) \right)  \label{A4bound} \\
|\tilde{A}_4(\lambda)(b, c, d)| &\leq C |\lambda| e^{-\alpha X_i} \left( |c| + (|\lambda| + e^{-\alpha X^*})^2  |d| \right) \label{tildeA4bound}
\end{align}

\begin{proof}
At $x = 0$, since $\Phi^u_-(0, 0; \lambda) = P^u(\lambda)$ and $\Phi^s_+(0, 0; \lambda) = P^s(\lambda)$, 
the fixed point equations \eqref{Zfpeq} become
\begin{align*}
Z_i^-&(0) = \Phi^s_{i,-}(0, -X_{i-1}; \lambda) P^i_-(-X_{i-1}, \lambda)^{-1} a_{i-1}^- + P^u(\lambda) b_i^- - \Phi^c_{i,-}(0, -X_{i-1}; \lambda) P^i_-(-X_{i-1}, \lambda)^{-1} a_{i-1}^c \\
&+ \int_{-X_{i-1}}^0 \Phi^s_{i,-}(0, y; \lambda) P^i_-(y; \lambda)^{-1}[ c_{i-1} e^{\nu(\lambda)X_{i-1}} G_i^-(y) V^-(y; \lambda) + \lambda^2 d_i \tilde{H}_i^-(y)] dy \\
&+ \int_{-X_{i-1}}^0 \Phi^c_{i,-}(0, y; \lambda) P^i_-(y; \lambda)^{-1}[ c_{i-1} e^{\nu(\lambda)X_{i-1}} G_i^-(y) V^-(y; \lambda) + \lambda^2 d_i \tilde{H}_i^-(y)] dy  \\
\end{align*}
and
\begin{align*}
Z_i^+&(0) = \Phi^u_{i,+}(0, X_i; \lambda) P^i_+(X_i, \lambda)^{-1} a_i^+ +  P^s(\lambda)b_i^+ + \Phi^c_{i,+}(0, X_i; \lambda) P^i_+(X_i, \lambda)^{-1} a_i^c \\
&+ \int_{X_i}^0 \Phi^u_{i,+}(0, y; \lambda) P^i_+(y; \lambda)^{-1} [ c_i e^{-\nu(\lambda)X_i} G_i^-(y)V^+(y; \lambda) + \lambda^2 d_i \tilde{H}_i^+(y)] dy \\
&+ \int_{X_i}^0 \Phi^c_{i,+}(0, y; \lambda) P^i_+(y; \lambda)^{-1} [ c_i e^{-\nu(\lambda)X_i} G_i^-(y)V^+(y; \lambda) + \lambda^2 d_i \tilde{H}_i^+(y)] dy 
\end{align*}
First, recall that at $Q(0)$, the tangent spaces to the stable and unstable manifold are given by
\begin{align*}
T_{Q(0)} W^u(0) &= \R Q'(0) \oplus Y^- \\
T_{Q(0)} W^s(0) &= \R Q'(0) \oplus Y^+
\end{align*}
Thus we have
\begin{align*}
P^-(0)^{-1} Q'(0) &= V^- \in E^u(0) \\
P^+(0)^{-1} Q'(0) &= V^+ \in E^s(0)
\end{align*}
Let
\begin{align*}
E^u(0) &= \C V^- \oplus E^- \\
E^s(0) &= \C V^+ \oplus E^+ \\
\end{align*}
Then we have
\begin{align*}
P^-(0)^{-1} Y^- = E^- \\
P^+(0)^{-1} Y^+ = E^+ \\
\end{align*}
We will use this to decompose $b_i^\pm$ uniquely as $b_i^\pm = x_i^\pm + y_i^\pm$, where $x_i^\pm \in \C V^\pm$ and $y_i^\pm \in E^\pm$. Since the evolution operators $\Phi(0, 0; \lambda)$ involve $\lambda$ but the projections we will be taking are for $\lambda = 0$, we will substitute
\begin{align*}
P^{s/u/c}(\lambda) &= P^{s/u/c}(0) + (P^{s/u/c}(\lambda) - P^{s/u/c}(0)),
\end{align*}
where the second term is order $\mathcal{O}(|\lambda|)$. This gives us
\begin{align*}
Z_i^-&(0) = x_i^- + y_i^- + (P^u(\lambda) - P^u(0))b_i^- \\
&+ \Phi^s_{i,-}(0, -X_{i-1}; \lambda) P^i_-(-X_{i-1}, \lambda)^{-1} a_{i-1}^- - \Phi^c_{i,-}(0, -X_{i-1}; \lambda) P^i_-(-X_{i-1}, \lambda)^{-1} a_{i-1}^c \\
&+ \int_{-X_{i-1}}^0 \Phi^s_{i,-}(0, y; \lambda) P^i_-(y; \lambda)^{-1}[ c_{i-1} e^{\nu(\lambda)X_{i-1}} G_i^-(y) V^-(y; \lambda) + \lambda^2 d_i \tilde{H}_i^-(y)] dy \\
&+ \int_{-X_{i-1}}^0 \Phi^c_{i,-}(0, y; \lambda) P^i_-(y; \lambda)^{-1}[ c_{i-1} e^{\nu(\lambda)X_{i-1}} G_i^-(y) V^-(y; \lambda) + \lambda^2 d_i \tilde{H}_i^-(y)] dy  \\
\end{align*}
and
\begin{align*}
Z_i^+&(0) = x_i^+ + y_i^+ + (P^s(\lambda) - P^s(0)) b_i^+ \\
&+\Phi^u_{i,+}(0, X_i; \lambda) P^i_+(X_i, \lambda)^{-1} a_i^+ + \Phi^c_{i,+}(0, X_i; \lambda) P^i_+(X_i, \lambda)^{-1} a_i^c \\
&+ \int_{X_i}^0 \Phi^u_{i,+}(0, y; \lambda) P^i_+(y; \lambda)^{-1} [ c_i e^{-\nu(\lambda)X_i} G_i^-(y)V^+(y; \lambda) + \lambda^2 d_i \tilde{H}_i^+(y)] dy \\
&+ \int_{X_i}^0 \Phi^c_{i,+}(0, y; \lambda) P^i_+(y; \lambda)^{-1} [ c_i e^{-\nu(\lambda)X_i} G_i^-(y)V^+(y; \lambda) + \lambda^2 d_i \tilde{H}_i^+(y)] dy 
\end{align*}
Finally, we apply the conjugation operators $P^i_\pm(0; \lambda)$ in \eqref{centercond2}. For the terms involving $b$, we substitute
\[
P^i_\pm(0; \lambda) = P^i_\pm(0; 0) + (P^i_\pm(0; \lambda) - P^i_\pm(0; 0)),
\]
where the second term is order $\mathcal{O}(|\lambda|)$, to obtain the expressions
\begin{align*}
P^i_-(0; \lambda) Z_i^-&(0) = P^i_-(0; 0)(x_i^- + y_i^-) + (P^i_-(0; \lambda) - P^i_-(0; 0))b_i^- + P^i_-(0; \lambda)(P^u(\lambda) - P^u(0))b_i^- \\
&+ P^i_-(0; \lambda) \Phi^s_{i,-}(0, -X_{i-1}; \lambda) P^i_-(-X_{i-1}, \lambda)^{-1} a_{i-1}^- - P^i_-(0; \lambda) \Phi^c_{i,-}(0, -X_{i-1}; \lambda) P^i_-(-X_{i-1}, \lambda)^{-1} a_{i-1}^c \\
&+ P^i_-(0; \lambda) \int_{-X_{i-1}}^0 \Phi^s_{i,-}(0, y; \lambda) P^i_-(y; \lambda)^{-1}[ c_{i-1} e^{\nu(\lambda)X_{i-1}} G_i^-(y) V^-(y; \lambda) + \lambda^2 d_i \tilde{H}_i^-(y)] dy \\
&+ P^i_-(0; \lambda) \int_{-X_{i-1}}^0 \Phi^c_{i,-}(0, y; \lambda) P^i_-(y; \lambda)^{-1}[ c_{i-1} e^{\nu(\lambda)X_{i-1}} G_i^-(y) V^-(y; \lambda) + \lambda^2 d_i \tilde{H}_i^-(y)] dy  \\
\end{align*}
and
\begin{align*}
P^i_+(0; \lambda) Z_i^+&(0) = P^i_+(0; 0)(x_i^+ + y_i^+) + (P^i_+(0; \lambda) - P^i_+(0; 0))b_i^+ + P^i_+(0; \lambda) (P^s(\lambda) - P^s(0)) b_i^+ \\
&+ P^i_+(0; \lambda) \Phi^u_{i,+}(0, X_i; \lambda) P^i_+(X_i, \lambda)^{-1} a_i^+ + P^i_+(0; \lambda) \Phi^c_{i,+}(0, X_i; \lambda) P^i_+(X_i, \lambda)^{-1} a_i^c \\
&+ P^i_+(0; \lambda) \int_{X_i}^0 \Phi^u_{i,+}(0, y; \lambda) P^i_+(y; \lambda)^{-1} [ c_i e^{-\nu(\lambda)X_i} G_i^-(y)V^+(y; \lambda) + \lambda^2 d_i \tilde{H}_i^+(y)] dy \\
&+ P^i_+(0; \lambda) \int_{X_i}^0 \Phi^c_{i,+}(0, y; \lambda) P^i_+(y; \lambda)^{-1} [ c_i e^{-\nu(\lambda)X_i} G_i^-(y)V^+(y; \lambda) + \lambda^2 d_i \tilde{H}_i^+(y)] dy 
\end{align*}
With this setup, the projections on $\C Q'(0)$ and $Y^+ \oplus Y^-$ will either eliminate or act as the identity on the terms $P^i_\pm(0; 0)(x_i^\pm + y_i^\pm$ in the first lines of $P^i_\pm(0; \lambda) Z_i^\pm(0)$. Applying the projections in \eqref{centercond2}, we obtain an expression of the form
\begin{equation}\label{projxy}
\begin{pmatrix}x_i^- \\ x_i^+ \\ 
y_i^+ - y_i^- \end{pmatrix} + L_4(\lambda)_i(b, c, d) = 0
\end{equation}
To get a bound on $L_4$, we will bound the individual terms involved. 

\begin{enumerate}
\item For the $a_i^\pm$ terms, we use the bound for $A_1$ from \cref{Zinv1} and the exponential trichotomy bounds \cref{Zevolbounds} to get
\begin{align*}
|P^i_+(0; \lambda) \Phi^u(0, X_i; \lambda) P^i_+(X_i, \lambda)^{-1} a_i^+| 
&\leq C e^{-\alpha X^*} \left( e^{-\alpha X^*} |b| + (e^{-\alpha X^*} + |C_i|)|c| + |\lambda|^2 |d| + |D_i||d| \right)
\end{align*}
The term involving $a_{i-1}^-$ is similar.

\item For the $a_i^c$ terms, we use the expression from Lemma \ref{lemma:aipm} and the exponential trichotomy bound \cref{Zevolbounds} to get
\begin{align*}
|P^i_+(0; \lambda) \Phi^c_{i,+}(0, X_i; \lambda) P^i_+(X_i, \lambda)^{-1} a_i^c| &\leq C |\lambda| e^{-(\alpha - \eta) X_i} \left( e^{-\alpha X^*}  |b| + |c| +|\lambda|^2 |d| \right)
\end{align*}
The term involving $a_{i-1}^c$ is similar. 

\item For the remainder terms involving $b_i$, since the conjugation operators $P^i_\pm(x; \lambda)$ and eigenprojections $P^{s/u}(\lambda)$ are smooth in $\lambda$, we have
\begin{align*}
|(P^i_+(0; \lambda) - P^i_+(0; 0))b_i^+ + P^i_+(0; \lambda) (P^s(\lambda) - P^s(0)) b_i^+| \leq C |\lambda| |b|
\end{align*}
The $b_i^-$ term is similar.

\item The bound on the integral terms is determined by the integrals involving the center subspace, since the other integrals will have stronger bounds. For the integrals involving $\tilde{H}_i^\pm$, we use the bounds from \cref{stabestimateslemma} together with the exponential trichotomy bound \cref{Zevolbounds} to get
\begin{align*}
&\left| P^i_+(0; \lambda) \int_{X_i}^0 \Phi^c_{i,+}(0, y; \lambda) P^i_+(y; \lambda)^{-1} \lambda^2 d_i \tilde{H}_i^+(y) dy \right| \leq C |\lambda|^2 |d| \int_0^{X_i} e^{-\alpha y} dy \leq C |\lambda|^2 |d|
\end{align*}
For the integrals involving $G_i^\pm(x)$, using \cref{stabestimateslemma}, the definition of $V^+(y; \lambda)$, and the center evolution \cref{centerevol},
\begin{align*}
&\left| P^i_+(0; \lambda) \int_{X_i}^0 \Phi^c_{i,+}(0, y; \lambda) P^i_+(y; \lambda)^{-1} c_i e^{-\nu(\lambda)X_i} G_i^-(y)V^+(y; \lambda) dy \right| \\
&\leq C |c| \left| e^{-\nu(\lambda)X_i} \right| \int_0^{X_i} e^{-\alpha X_i} e^{-\alpha(X_i - y) } + e^{-2 \alpha X_{i-1}} e^{-\alpha y} dy \\
&\leq C e^{-\alpha X^*} |c|,
\end{align*}
where we bounded $e^{-\nu(\lambda)X_i}$ by a constant using \cref{lemma:expnubound}.
\end{enumerate}

Combining all of these individual bounds, using the estimate $|D_i| \leq C e^{-\alpha X^*}$, and simplifying, we obtain the uniform bound for $L_4(\lambda)(b, c, d)$.
\begin{align*}
L_4(\lambda)(b, c, d) \leq 
C\Big( (|\lambda| + e^{-\alpha X^*})|b| + e^{-\alpha X^*}|c| + (|\lambda| + e^{-\alpha X^*})^2 |d|  \Big) 
\end{align*}
Since $|\lambda| < \delta$ and $e^{-\alpha X^*} < \delta$, this becomes
\begin{align*}
L_4(\lambda)(b, c, d) \leq 
C\Big( \delta |b| + e^{-\alpha X^*}|c| + (|\lambda| + e^{-\alpha X^*})^2 |d| \Big) 
\end{align*}
which is uniform in $|b|$. Define the map
\[
J_2: \left( \bigoplus_{j=1}^n \C V^+ \oplus \C V^- \right) \oplus
\left( \bigoplus_{j=1}^n E^+ \oplus E^- \right) 
\rightarrow \bigoplus_{j=1}^n \C V^+ \oplus \C V^- \oplus (E^+ \oplus E^-)
\]
by 
\[
J_2( (x_i^+, x_i^-),(y_i^+, y_i^-))_i = ( x_i^+, x_i^-, y_i^+ - y_i^- )
\]
Since $\C^{2m} = E^s(0) \oplus E^u(0) = \C V^+ \oplus \C V^- \oplus (E^+ \oplus E^-)$, $J_2$ is an isomorphism. Using this and the fact that $b_i = (x_i^- + y_i^-, x_i^+ + y_i^+)$, we can write \eqref{projxy} as
\begin{equation}\label{projxy2}
J_2( (x_i^+, x_i^-),(y_i^+, y_i^-))_i 
+ L_4(\lambda)_i(b_i, 0, 0) + L_4(\lambda)_i(0, c, d) = 0
\end{equation}
Consider the map
\begin{align*}
S_2(b)_i &= J_2( (x_i^+, x_i^-),(y_i^+, y_i^-))_i 
+ L_4(\lambda)_i(b_i, 0, 0) 
\end{align*}
Substituting this in \eqref{projxy2}, we have
\begin{align*}
S_2(b) &= -L_4(\lambda)(0, c, d)
\end{align*}

Decreasing $\delta$ if necessary, the operator $S_2(b)$ is invertible. Thus we can solve for $b$ to get
\begin{align}
b = B_1(\lambda)(c,d) 
= -S_2^{-1} L_4(\lambda)(0, c, d)
\end{align}
The bound on $B_1$ is given by the bound on $L_4$.
\begin{align*}
|B_1(\lambda)(c, d)| \leq C\Big( e^{-\alpha X^*}|c| + (|\lambda| + e^{-\alpha X^*})^2 |d| \Big) 
\end{align*}
We now plug $B_1$ into all of the previous bounds, using in addition the bound on $C_i c$ from Lemma \ref{stabestimateslemma} and $D_i d = \mathcal{O}(e^{-\alpha X^*}|d|)$. Plugging $B_1$ into the bound \eqref{A1bound} for $A_1$, we get $A_3$ with bound given by \cref{A3bound}. Plugging $B_1$ into the bound \eqref{A2bound} for $A_2$, we get $A_4$ with bound \cref{A4bound}. Finally, we plug in $B_1$ into the bound for $\tilde{A}_2$ to get $\tilde{A}_4$ with bound \cref{tildeA4bound}.
\end{proof}
\end{lemma}

\section{Jump Conditions}

Up to this point, we have solved uniquely for $a$ and $b$. We will not be able to obtain a unique solution for $c$ and $d$. We will instead compute jump conditions in the direction of $\Psi(0)$ and $\Psi^c(0)$. Obtaining a nontrivial solution for $c$ and $d$ will be equivalent to these jump conditions being 0. First, we compute the jump in the direction of $\Psi^c(0)$. 

% jump lemma : center adjoint
\begin{lemma}\label{jumpcenteradj}
The jumps in the direction of $\Psi^c(0)$ are given by
\begin{equation}\label{xic}
\begin{aligned}
\xi^c_i &= e^{-\nu(\lambda)X_i} c_i - e^{\nu(\lambda)X_i} c_{i-1} - \frac{1}{2}\lambda \tilde{M} \left( e^{-\nu(\lambda)X_i}c_i + e^{\nu(\lambda)X_i}c_{i-1}\right) - \lambda^2 \tilde{M}^c d_i + R^c(\lambda)_i(c, d)
\end{aligned}
\end{equation}
where
\begin{align*}
\tilde{M}^c &= \int_{-\infty}^\infty \partial_c q(y) dy \\
\tilde{M} &= \int_{-\infty}^{\infty} \left(v^c(y) - \frac{1}{c}\right) dy
\end{align*}
The remainder term $R^c_i(c, d)$ is analytic in $\lambda$ and linear in $(c, d)$ and has uniform bound \cref{centerR} given below in the proof. The jump conditions can be written in matrix form as
\begin{equation}\label{matrixjumpc}
\left( K(\lambda) -\frac{1}{2} \lambda \tilde{M} K_1(\lambda) + C_1 \right) c + (-\lambda^2 \tilde{M}^c I + D_1) d = 0.
\end{equation}
$K(\lambda)$ is the matrix
\begin{align*}
K(\lambda) =  
\begin{pmatrix}
e^{-\nu(\lambda)X_1} & & & & & -e^{\nu(\lambda)X_0} \\
-e^{\nu(\lambda)X_1} & e^{-\nu(\lambda)X_2} \\
& -e^{\nu(\lambda)X_2} & e^{-\nu(\lambda)X_3} \\
  & & \ddots & && \\
& & & & -e^{\nu(\lambda)X_{n-1}} & e^{-\nu(\lambda)X_0}
\end{pmatrix},
\end{align*}
$K_1(\lambda)$ is the matrix
\begin{align*}
K_1(\lambda) =  
\begin{pmatrix}
e^{-\nu(\lambda)X_1} & & & & & e^{\nu(\lambda)X_0} \\
e^{\nu(\lambda)X_1} & e^{-\nu(\lambda)X_2} \\
& e^{\nu(\lambda)X_2} & e^{-\nu(\lambda)X_3} \\
 & & \ddots & &&   \\
& & & & e^{\nu(\lambda)X_{n-1}} & e^{\nu(\lambda)X_0}
\end{pmatrix},
\end{align*}
The remainder matrices have uniform bounds
\begin{align}\label{centerjumprem}
|C_1| &\leq C |\lambda|(|\lambda| + r^{1/2}) \\
|D_1| &\leq C |\lambda|(|\lambda| + r^{1/2})^2
\end{align}

\begin{proof}
We want to solve the center jump conditions, which are given by
\[
\xi_i^c = 
\langle \Psi^c(0), P^i_+(0; \lambda) Z_i^+(0) - P^i_-(0; \lambda) Z_i^-(0) + c_i e^{-\nu(\lambda)X_i}V^+(0; \lambda) - c_{i-1} e^{\nu(\lambda)X_i} V^-(0; \lambda) \rangle 
\]
From \cref{lemma:VpmPsiIP},
\begin{align}\label{centerVjump}
\langle \Psi^c(0), &c_i e^{-\nu(\lambda)X_i}V^+(0; \lambda) - c_{i-1} e^{\nu(\lambda)X_i} V^-(0; \lambda) \rangle \\
&= e^{-\nu(\lambda)X_i}c_i  - e^{\nu(\lambda)X_i}c_{i-1} 
-\frac{1}{2}\lambda \tilde{M} \left( e^{-\nu(\lambda)X_i}c_i + e^{\nu(\lambda)X_i}c_{i-1}\right)+ \mathcal{O}(|\lambda|^2 |c| ),
\end{align}
where we used Lemma \ref{lemma:expnubound} to bound $e^{\pm\nu(\lambda)X_i}$ in the remainder term by a constant. The terms $P^i_\pm(0; \lambda) Z_i^\pm(0)$ are given by
\begin{align*}
P^i_-(0; \lambda) Z_i^-&(0) = P^i_-(0; 0) b_i^- + (P^i_-(0; \lambda) - P^i_-(0; 0))b_i^- + P^i_-(0; \lambda)(P^u(\lambda) - P^u(0))b_i^- \\
&+ P^i_-(0; \lambda) \Phi^s_{i,-}(0, -X_{i-1}; \lambda) P^i_-(-X_{i-1}, \lambda)^{-1} a_{i-1}^- - P^i_-(0; \lambda) \Phi^c_{i,-}(0, -X_{i-1}; \lambda) P^i_-(-X_{i-1}, \lambda)^{-1} a_{i-1}^c \\
&+ P^i_-(0; \lambda) \int_{-X_{i-1}}^0 \Phi^s_{i,-}(0, y; \lambda) P^i_-(y; \lambda)^{-1}[ c_{i-1} e^{\nu(\lambda)X_{i-1}} G_i^-(y) V^-(y; \lambda) + \lambda^2 d_i \tilde{H}_i^-(y)] dy \\
&+ P^i_-(0; \lambda) \int_{-X_{i-1}}^0 \Phi^c_{i,-}(0, y; \lambda) P^i_-(y; \lambda)^{-1}[ c_{i-1} e^{\nu(\lambda)X_{i-1}} G_i^-(y) V^-(y; \lambda) + \lambda^2 d_i \tilde{H}_i^-(y)] dy  \\
\end{align*}
and
\begin{align*}
P^i_+(0; \lambda) Z_i^+&(0) = P^i_+(0; 0)b_i^+ + (P^i_+(0; \lambda) - P^i_+(0; 0))b_i^+ + P^i_+(0; \lambda) (P^s(\lambda) - P^s(0)) b_i^+ \\
&+ P^i_+(0; \lambda) \Phi^u_{i,+}(0, X_i; \lambda) P^i_+(X_i, \lambda)^{-1} a_i^+ + P^i_+(0; \lambda) \Phi^c_{i,+}(0, X_i; \lambda) P^i_+(X_i, \lambda)^{-1} a_i^c \\
&+ P^i_+(0; \lambda) \int_{X_i}^0 \Phi^u_{i,+}(0, y; \lambda) P^i_+(y; \lambda)^{-1} [ c_i e^{-\nu(\lambda)X_i} G_i^-(y)V^+(y; \lambda) + \lambda^2 d_i \tilde{H}_i^+(y)] dy \\
&+ P^i_+(0; \lambda) \int_{X_i}^0 \Phi^c_{i,+}(0, y; \lambda) P^i_+(y; \lambda)^{-1} [ c_i e^{-\nu(\lambda)X_i} G_i^-(y)V^+(y; \lambda) + \lambda^2 d_i \tilde{H}_i^+(y)] dy 
\end{align*}

The only leading order term involves the center integral involving $\tilde{H}_i^\pm$. Using \cref{Zevolmod} for $\Phi^c_{i,-}$, this becomes
\begin{align*}
\langle W_0, &P^i_-(0; \lambda) \lambda^2 d_i \int_{-X_{i-1}}^0 \Phi^c_{i,-}(0, y; \lambda) P^i_-(y; \lambda)^{-1} \tilde{H}_i^-(y) dy \rangle \\
&= \lambda^2 d_i \int_{-X_{i-1}}^0 \langle W_0, P^i_-(0; \lambda) \Phi(0, -X_{i-1}; \lambda) P^i_-(-X_{i-1}, \lambda)^{-1} \\
&\qquad \qquad
P^c(0) P^i_-(-X_{i-1}, \lambda) \Phi(-X_{i-1}, y; \lambda) P^i_-(y; \lambda)^{-1} \tilde{H}_i^-(y) \rangle dy \\
&= \lambda^2 d_i \int_{-X_{i-1}}^0 \langle W_0, \tilde{\Phi}_-(0, -X_{i-1}; \lambda) 
P^c(0) \tilde{\Phi}_-(-X_{i-1}, y; \lambda) \tilde{H}_i^-(y) \rangle dy \\ 
&= \lambda^2 d_i \int_{-X_{i-1}}^0 \langle W_0, \tilde{\Phi}_-(0, -X_{i-1}; 0) 
P^c(0) \tilde{\Phi}_-(-X_{i-1}, y; 0) H(y) \rangle dy + \mathcal{O}(|\lambda|^3 |d|) \\
&= \lambda^2 d_i \int_{-X_{i-1}}^0 \langle \tilde{\Phi}^*_-(y, -X_{i-1}; 0) [P^c(0)]^* \tilde{\Phi}^*_-(-X_{i-1}, 0; 0) W_0,
 H(y) \rangle dy + \mathcal{O}(|\lambda|^3 |d|) \\
&= \lambda^2 d_i \int_{-X_{i-1}}^0 \langle \tilde{\Phi}^*_-(y, -X_{i-1}; 0) P^{c,*}(0) \tilde{\Phi}^*_-(-X_{i-1}, 0; 0) W_0,
 H(y) \rangle dy + \mathcal{O}(|\lambda|^3 |d|) \\
&= \lambda^2 d_i \int_{-X_{i-1}}^0 \langle W_0, H(y) \rangle dy + \mathcal{O}(|\lambda|^3 |d|) \\
&= \lambda^2 d_i \int_{-\infty}^0 \langle W_0, H(y) \rangle dy + \mathcal{O}(|\lambda|^3 |d|)
\end{align*}
since $\tilde{\Phi}^*(y, x; 0)$ is the evolution equation for the adjoint variational equation, $W_0$ is a constant solution to this equation, and $P^{c,*}(0) W_0 = W_0$. Since $H(y) = B \partial_c Q(y)$,
\begin{align*}
\langle W_0, &P^i_-(0; \lambda) \lambda^2 d_i \int_{-X_{i-1}}^0 \Phi^c_{i,-}(0, y; \lambda) P^i_-(y; \lambda)^{-1} \tilde{H}_i^-(y) dy \rangle 
= \lambda^2 d_i \int_{-\infty}^0 \partial_c q(y)dy + \mathcal{O}(|\lambda|^3 |d|)
\end{align*}
Similary, 
\begin{align*}
\langle W_0, &P^i_+(0; \lambda) \lambda^2 d_i \int_{X_i}^0 \Phi^c_{i,+}(0, y; \lambda) P^i_+(y; \lambda)^{-1}   \tilde{H}_i^+(y) \rangle 
= -\lambda^2 d_i \int_0^{\infty} \partial_c q(y)dy + \mathcal{O}(|\lambda|^3 |d|)
\end{align*}

The rest of the terms are higher order.
\begin{enumerate}
\item For the terms involving $a_i^\pm$, we use the definitions of $\Phi^u_{i,+}$ and $\Phi^s_{i,i}$, \cref{Zevolbounds}, and the bound for $A_3$ from \cref{Zinv2} to get
\begin{align*}
\langle W_0, &P^i_+(0; \lambda) \Phi^u_{i,+}(0, X_i; \lambda) P^i_+(X_i, \lambda)^{-1} a_i^+ \rangle = \langle W_0, \tilde{\Phi}_+(0, X_i; \lambda) 
P^u(0) \tilde{\Phi}_+(X_i, X_i; \lambda)a_i^+ \rangle \\
&= \langle W_0, P^u(0) a_i^+ \rangle + \mathcal{O}(|\lambda|e^{-\alpha X_*}|a_i^+|) \\
&= \langle \tilde{\Phi}^*_+(X_i, 0; 0) W_0, P^u(0) a_i^+ \rangle + \mathcal{O}(|\lambda|e^{-\alpha X_*}|a_i^+|) \\
&= \langle W_0, P^u(0) a_i^+ \rangle + \mathcal{O}(|\lambda|e^{-\alpha X_*}|a_i^+|) \\
&= \mathcal{O}\left(|\lambda|e^{-\alpha X_*} \left( e^{-\alpha X^*} |c| + |\lambda|^2 |d| + |D_i||d| \right) \right)
\end{align*}
The term involving $a_{i-1}^-$ is similar.

\item For the terms involving $a_i^c$, we use the definitions of $\Phi^c_{i,\pm}$, \cref{Zevolbounds} and the bound for $\tilde{A}_4$ from \cref{Zinv2} to get
 to get
\begin{align*}
\langle W_0, &P^i_+(0; \lambda) \Phi^c_{i,+}(0, X_i; \lambda) P^i_+(X_i, \lambda)^{-1} a_i^c \rangle = \langle W_0, \tilde{\Phi}_+(0, X_i; \lambda) 
P^c(0) \tilde{\Phi}_+(X_i, X_i; \lambda)a_i^c \rangle \\
&= \langle \tilde{\Phi}^*_+(X_i, 0; 0) W_0, P^u(0) a_i^c \rangle + \mathcal{O}(|\lambda|e^{\eta X_i}|a_i^c|) \\
&= \langle W_0, a_i^c \rangle + \mathcal{O}(|\lambda|e^{\eta X_i}|a_i^c|) \\
\end{align*}
Thus we have
\begin{align*}
&\left| \langle W_0, P^i_+(0; \lambda) \Phi^c_{i,+}(0, X_i; \lambda) P^i_+(X_i, \lambda)^{-1} a_i^c \rangle \right| \leq C |a_i^c| \\
&\qquad\leq C |\lambda|(e^{-\alpha X^*} + |\lambda|) \left( |c| + (|\lambda| + e^{-\alpha X^*})^2  |d| \right)
\end{align*}
The term involving $a_{i-1}^c$ is similar.

\item For the terms involving $b$, the terms $P_-(0; 0) b_i^-$ and $P_+(0, 0)b_i^+$ are eliminated outright when we take the inner product with $W_0$. For the other terms, we use the estimate for $B_1$ from Lemma \ref{Zinv2}.
\begin{align*}
\left| \langle W_0, (P^i_+(0; \lambda) - P^i_+(0; 0))b_i^+ + P^i_+(0; \lambda) (P^s(\lambda) - P^s(0)) b_i^+ \rangle \right| \leq C |\lambda| \left( e^{-\alpha X^*}|c| + (|\lambda| + e^{-\alpha X^*})^2 |d| \right)
\end{align*}
The $b_i^-$ term is similar.

\item For the center integrals involving $G_i^\pm$, we follow the same procedure as the center integrals involving $\tilde{H}_i^\pm$ and use the bound on this integral from \cref{Zinv2} to get
\begin{align*}
\langle W_0, &P^i_-(0; \lambda) \int_{-X_{i-1}}^0 \Phi^c_{i,-}(0, y; \lambda) P^i_-(y; \lambda)^{-1} c_{i-1} e^{\nu(\lambda)X_{i-1}} G_i^-(y) V^-(y; \lambda) dy \rangle \\
&= c_{i-1} e^{\nu(\lambda)X_{i-1}}\int_{-\infty}^0 \langle W_0, G_i^-(y) V^-(y; \lambda)  \rangle dy + \mathcal{O}(|\lambda| e^{-\alpha X^*} |c|) \\
&= \mathcal{O}(|\lambda| e^{-\alpha X^*} |c|)
\end{align*}
where we bounded $e^{\nu(\lambda)X_{i-1}}$ by a constant in the remainder term. The inner product in the integrand is 0 since the bottom row of $G_i^\pm(y)$ is all zeros. The other center integral term is similar.

\item For the noncenter integral involving $\tilde{H}_i^\pm$, we follow the same procedure as with the center integral involving $\tilde{H}_i^\pm$, except $P^c(0)$ is replaced with $P^{s/u}(0)$. Thus for both cases, the integrals are $\mathcal{O}(|\lambda|^3)$. The bound for the noncenter integral involving $G_i^\pm(x) V^\pm(x)$ is stronger than the bound for the center integral involving $G_i^\pm(x) V^\pm(x)$, thus is subsumed by that bound.
\end{enumerate}

We put this all together to obtain the center jump expressions, which are given by
\begin{align*}
\xi^c_i &= e^{-\nu(\lambda)X_i} c_i - e^{\nu(\lambda)X_i} c_{i-1} - \frac{1}{2}\lambda \tilde{M} \left( e^{-\nu(\lambda)X_i}c_i + e^{\nu(\lambda)X_i}c_{i-1}\right) -\lambda^2 \tilde{M}^c d_i + R^c(\lambda)_i(c, d)
\end{align*}
where
\begin{align*}
\tilde{M}^c &= \int_{-\infty}^\infty \partial_c q(y) dy \\
\tilde{M} &= \int_{-\infty}^{\infty} \left(v^c(y) - \frac{1}{c}\right) dy
\end{align*}
and the remainder term $R^c_i(c, d)$ has uniform bound
\begin{equation}\label{centerR}
\begin{aligned}
\|R^c&(c, d)\| \leq C \Big( |\lambda| (e^{-\alpha X^*} + |\lambda|) |c| + |\lambda| (|\lambda| + e^{-\alpha X^*})^2 |d| \Big)
\end{aligned}
\end{equation}

Finally, we write this in matrix form. The leading order terms involving $c$ are given by $K(\lambda)c -\frac{1}{2} \lambda \tilde{M} K_1(\lambda) c$, where $K(\lambda)$ and $K_1(\lambda)$ are the periodic, bi-diagonal matrices
\begin{align*}
K(\lambda) =  
\begin{pmatrix}
e^{-\nu(\lambda)X_1} & & & & & -e^{\nu(\lambda)X_0} \\
-e^{\nu(\lambda)X_1} & e^{-\nu(\lambda)X_2} \\
& -e^{\nu(\lambda)X_2} & e^{-\nu(\lambda)X_3} \\
  & & \ddots & && \\
& & & & -e^{\nu(\lambda)X_{n-1}} & e^{-\nu(\lambda)X_0}
\end{pmatrix},
\end{align*}
\begin{align*}
K_1(\lambda) =  
\begin{pmatrix}
e^{-\nu(\lambda)X_1} & & & & & e^{\nu(\lambda)X_0} \\
e^{\nu(\lambda)X_1} & e^{-\nu(\lambda)X_2} \\
& e^{\nu(\lambda)X_2} & e^{-\nu(\lambda)X_3} \\
 & & \ddots & &&   \\
& & & & e^{\nu(\lambda)X_{n-1}} & e^{\nu(\lambda)X_0}
\end{pmatrix},
\end{align*}
and $c = (c_1, \dots, c_{n-1}, c_0)^T$. The leading order terms involving $d$ is the diagonal matrix $-\lambda^2 \tilde{M}^c I$. Let $C_1$ and $D_1$ be the matrices we get from the remainder terms involving $c$ and $d$. Since $e^{-\alpha X^*} = C r^{1/2}$, $C_1$ and $D_1$ have the bounds in \cref{centerjumprem}. Similarly, using \cref{lemma:expnubound} to bound the terms of the form $e^{\pm \nu(\lambda)X_j}$, $K_2(\lambda)$ has the bound in \cref{centerjumprem}, which is uniform in $\lambda$. Combining everything, the center jump condition can be written in matrix form as \cref{matrixjumpc}.
\end{proof}
\end{lemma}

Finally, we compute the jump in the direction of $\Psi(0)$.

% lemma : jump in decaying adjoint direction
\begin{lemma}\label{jumpadj}
The jumps in the direction of $\Psi(0)$ are given by
\begin{equation}\label{jumpPsi0}
\begin{aligned}
\xi_i = \langle \Psi&(X_i), Q'(-X_i) \rangle (d_{i+1} - d_i ) + \langle \Psi(-X_{i-1}), Q'(X_{i-1}) \rangle (d_i - d_{i-1} ) \\
&-\frac{1}{2}\lambda M^c\left( e^{-\nu(\lambda)X_i}c_i + e^{\nu(\lambda)X_i}c_{i-1}\right)
- \lambda^2 d_i M + R_i(\lambda)(c, d)
\end{aligned}
\end{equation}
$M$ is the higher order Melnikov integral
\begin{equation}\label{defM2}
M = \int_{-\infty}^\infty \langle \Psi(y), B H(y) \rangle dy
\end{equation}
and $M^c$ is the center Melnikov integral defined in \cref{lemma:VderivIPs}. The remainder term $R(\lambda)(c, d)$ is analytic in $\lambda$, linear in $(c, d)$, and has bound given by \cref{noncenterR} in the proof below. The jump conditions can be written in matrix form as
\begin{equation}\label{Psimatrix}
\left(-\frac{1}{2} \lambda M^c K_1(\lambda) + C_2 \right)c + (A - \lambda^2 M I + D_2)d = 0.
\end{equation}
The matrix $A$ is given by
\begin{align*}
A &= \begin{pmatrix}
-a_0 -a_1 & a_0 + a_1  \\
-a_0 + a_1 & -a_0 - a_1
\end{pmatrix} && n = 2 \\
A &= \begin{pmatrix}
-a_{n-1} - a_0 & a_0 & & & \dots & a_{n-1}\\
a_0 & -a_0 - a_1 &  a_1   \\
& a_1 & -a_1 - a_2 &  a_2 \\
& & \vdots & & \vdots \\
a_{n-1} & & & & a_{n-2} & -a_{n-2} - a_{n-1} \\
\end{pmatrix} && n > 2
\end{align*}
with
\begin{align*}
a_i &= \langle \Psi(X_i), Q'(-X_i) \rangle \\
\end{align*}
The matrix $K_1(\lambda)$ is given by
\begin{align*}
K_1(\lambda) =  
\begin{pmatrix}
e^{-\nu(\lambda)X_1} & & & & & e^{\nu(\lambda)X_0} \\
e^{\nu(\lambda)X_1} & e^{-\nu(\lambda)X_2} \\
& e^{\nu(\lambda)X_2} & e^{-\nu(\lambda)X_3} \\
 & & \ddots & &&   \\
& & & & e^{\nu(\lambda)X_{n-1}} & e^{\nu(\lambda)X_0}
\end{pmatrix}
\end{align*}
The remainder matrices have uniform bounds
\begin{align}\label{adjjumprem}
|C_2| &\leq C (|\lambda| + r^{1/2})^2 \\
|D_2| &\leq C (|\lambda| + r^{1/2})^3 
\end{align}

\begin{proof}
We want to solve the decaying adjoint jump condition, which is given by
\[
\xi_i = 
\langle \Psi(0), P^i_+(0; \lambda) Z_i^+(0) - P^i_-(0; \lambda) Z_i^-(0) + c_i e^{-\nu(\lambda)X_i}V^+(0; \lambda) - c_{i-1} e^{\nu(\lambda)X_i} V^-(0; \lambda) \rangle 
\]
From \cref{lemma:VpmPsiIP},
\begin{align}\label{PsiVpmjump}
\langle \Psi^c(0), c_i e^{-\nu(\lambda)X_i}V^+(0; \lambda) - c_{i-1} e^{\nu(\lambda)X_i} V^-(0; \lambda)  \rangle &= -\frac{1}{2}\lambda M^c\left( e^{-\nu(\lambda)X_i}c_i + e^{\nu(\lambda)X_i}c_{i-1}\right) + \mathcal{O}(|\lambda|^2 |c| ),
\end{align}
where we used Lemma \ref{lemma:expnubound} to bound $e^{\pm\nu(\lambda)X_i}$ in the remainder term by a constant. The terms $P^i_\pm(0; \lambda) Z_i^\pm(0)$ are given in the proof of the previous lemma. As in Lemma \ref{jumpcenteradj}, we begin by computing the leading order terms.

\begin{enumerate}
\item The non-center integral will give us the higher order Melnikov integral. For the piece on $\R^-$ we use the uniform estimate $\tilde{H}_i^-(y) = H(y) + \mathcal{O}(e^{-\alpha X^*})$ from Lemma \ref{stabestimateslemma} and the definition of    to get
\begin{align*}
&\langle \Psi(0), P^i_-(0; \lambda) \int_{-X_{i-1}}^0 \Phi^s_{i,-}(0, y; \lambda) P^i_-(y; \lambda)^{-1} \lambda^2 d_i \tilde{H}_i^-(y) dy \rangle \\
&= \lambda^2 d_i \int_{-X_{i-1}}^0 \langle \Psi(0), \tilde{\Phi}_-(0, -X_{i-1}; \lambda) 
P^s(0) \tilde{\Phi}_-(-X_{i-1}, y; \lambda) H(y) \rangle dy + \mathcal{O}(|\lambda|^2( |\lambda| + {e^{-\alpha X^*}})|d|) \\
&= \lambda^2 d_i \int_{-X_{i-1}}^0 \langle \Psi(0), \tilde{\Phi}_-(0, -X_{i-1}; 0) 
P^s(0) \tilde{\Phi}_-(-X_{i-1}, y; 0) H(y) \rangle dy + \mathcal{O}(|\lambda|^2( |\lambda| + {e^{-\alpha X^*}})|d|) \\
&= \lambda^2 d_i \int_{-X_{i-1}}^0 \langle \tilde{\Phi}^*_-(y, -X_{i-1}; 0) [P^s(0)]^* \tilde{\Phi}^*_-(-X_{i-1}, 0; 0) \Psi(0), H(y) \rangle dy + \mathcal{O}(|\lambda|^2( |\lambda| + {e^{-\alpha X^*}})|d|) \\
&= \lambda^2 d_i \int_{-X_{i-1}}^0 \langle \tilde{\Phi}^*_-(y, -X_{i-1}; 0) P^{u,*}(0) \Psi(-X_{i-1}), H(y) \rangle dy + \mathcal{O}(|\lambda|^2( |\lambda| + {e^{-\alpha X^*}})|d|)
\end{align*}
Since $P^{u,*}(0) \Psi(-X_{i-1}) = \Psi(-X_{i-1}) + \mathcal{O}(e^{-2\alpha X_{i-1}})$, this becomes
\begin{align*}
&\langle \Psi(0), P^i_-(0; \lambda) \int_{-X_{i-1}}^0 \Phi^s_{i,-}(0, y; \lambda) P^i_-(y; \lambda)^{-1} \lambda^2 d_i \tilde{H}_i^-(y) dy \rangle \\
&= \lambda^2 d_i \int_{-X_{i-1}}^0 \langle \tilde{\Phi}^*_-(y, -X_{i-1}; 0) \Psi(-X_{i-1}), H(y) \rangle dy + \mathcal{O}(|\lambda|^2( |\lambda| + {e^{-\alpha X^*}})|d|) \\
&= \lambda^2 d_i \int_{-X_{i-1}}^0 \langle \Psi(y), H(y) \rangle dy + \mathcal{O}(|\lambda|^2( |\lambda| + {e^{-\alpha X^*}})|d|) \\
\end{align*}
Since 
\[
\left| \int_{-\infty}^{-X_{i-1}} \langle \Psi(y), H(y) \rangle dy \right| \leq C e^{-\alpha X_{i-1}},
\]
we have
\begin{align*}
&\langle \Psi(0), P^i_-(0; \lambda) \int_{-X_{i-1}}^0 \Phi^s_{i,-}(0, y; \lambda) P^i_-(y; \lambda)^{-1} \lambda^2 d_i \tilde{H}_i^-(y) dy \rangle \\
&= \lambda^2 d_i \int_{-\infty}^0 \langle \Psi(y), H(y) \rangle dy + \mathcal{O}(|\lambda|^2( |\lambda| + {e^{-\alpha X^*}})|d|) \\
\end{align*}
Finally, we substitute $H(y) = B \partial_c Q(y)$ to get
\begin{align*}
&\langle \Psi(0), P^i_-(0; \lambda) \int_{-X_{i-1}}^0 \Phi^s_{i,-}(0, y; \lambda) P^i_-(y; \lambda)^{-1} \lambda^2 d_i \tilde{H}_i^-(y) dy \rangle \\
&= \lambda^2 d_i \int_{-\infty}^0 \langle \Psi(y), B \partial_c Q(y) \rangle dy + \mathcal{O}(|\lambda|^2( |\lambda| + {e^{-\alpha X^*}})|d|) \\
&= \lambda^2 d_i \int_{-\infty}^0 q(y) \partial_c q(y) dy + \mathcal{O}(|\lambda|^2( |\lambda| + {e^{-\alpha X^*}})|d|)
\end{align*}
The piece on $\R^+$ is similar, and gives us the other half of the Melnikov integral $M$.

\item For the terms involving $a_i^\pm$, we use the definitions of $\Phi^u_{i,+}$ and $\Phi^s_{i,i}$, the trichotomy estimates \cref{Zevolbounds}, and the bound $A_4$ from \cref{Zinv2} to get
\begin{align*}
\langle \Psi(0), &P^i_+(0; \lambda) \Phi^u_{i,+}(0, X_i; \lambda) P^i_+(X_i, \lambda)^{-1} a_i^+ \rangle = \langle \Psi(0), \tilde{\Phi}_+(0, X_i; \lambda) 
P^u(0) \tilde{\Phi}_+(X_i, X_i; \lambda)a_i^+ \rangle \\
&= \langle \tilde{\Phi}^*_+(X_i, 0; \lambda) \Psi(0), P^u(0) a_i^+ \rangle + \mathcal{O}(|\lambda|e^{-\alpha X_*}|a_i^+|) \\
&= \langle \Psi(X_i), P^u(0) a_i^+ \rangle + \mathcal{O}(|\lambda|e^{-\alpha X_*}|a_i^+|) \\
&= \langle \Psi(X_i), P^u(0) a_i^+ \rangle + \mathcal{O}\left(|\lambda|e^{-\alpha X_*} \left( e^{-\alpha X^*} |c| + |\lambda|^2 |d| + |D_i||d| \right) \right)
\end{align*}
Using the expression for $a_i^+$ from \cref{Zinv2} together with the bound for $A_4$ and simplifying, this becomes
\begin{align*}
\langle \Psi(0), &P^i_+(0; \lambda) \Phi^u_{i,+}(0, X_i; \lambda) P^i_+(X_i, \lambda)^{-1} a_i^+ \rangle \\
&= \langle \Psi(X_i), P^u(0) D_i d \rangle + \mathcal{O}\left(e^{-\alpha X_*} (e^{-\alpha X^*} + |\lambda|)|c| + e^{-\alpha X^*}(|\lambda| + e^{-\alpha X^*})^2 |d|  \right)
\end{align*}
Using the expression for $D_i d$ from \cref{stabestimateslemma}, 
\begin{align*} 
P^u(0) D_i d = Q'(-X_i)(d_{i+1} - d_i ) + \mathcal{O}( e^{-\alpha X_i} (e^{-\alpha X^*} + |\lambda| )|d|)
\end{align*}
Thus we have
\begin{align*}
\langle \Psi(0), &P^i_+(0; \lambda) \Phi^u_{i,+}(0, X_i; \lambda) P^i_+(X_i, \lambda)^{-1} a_i^+ \rangle \\
&= \langle \Psi(X_i), Q'(-X_i) \rangle (d_{i+1} - d_i ) + \mathcal{O}\left(e^{-\alpha X_*} (e^{-\alpha X^*} + |\lambda|)|c| + e^{-\alpha X^*}(|\lambda| + e^{-\alpha X^*})^2 |d|  \right)
\end{align*}
Similarly,
\begin{align*}
\langle \Psi(0), &P^i_-(0; \lambda) \Phi^s_{i,-}(0, -X_{i-1}; \lambda) P^i_-(-X_{i-1}, \lambda)^{-1} a_{i-1}^- \rangle \\
&= -\langle \Psi(-X_{i-1}), Q'(X_{i-1}) \rangle (d_i - d_{i-1} )
+ \mathcal{O}\left(e^{-\alpha X_*} (e^{-\alpha X^*} + |\lambda|)|c| + e^{-\alpha X^*}(|\lambda| + e^{-\alpha X^*})^2 |d|  \right)
\end{align*}

\end{enumerate}

The remaining terms will be higher order. As in the previous lemma, we will bound these in turn.
\begin{enumerate}
\item For the terms involving $a_i^c$, similar to \cref{jumpcenteradj}, we have
\begin{align*}
\langle \Psi(0), &P^i_+(0; \lambda) \Phi^c_{i,+}(0, X_i; \lambda) P^i_+(X_i, \lambda)^{-1} a_i^c \rangle = \langle \tilde{\Phi}^*_+(X_i, 0; 0) \Psi(0), P^u(0) a_i^c \rangle + \mathcal{O}(|\lambda|e^{\eta X_i}|a_i^c|) \\
&= \langle \Psi(X_i), a_i^c \rangle + \mathcal{O}(|\lambda|e^{\eta X_i}|a_i^c|) 
\end{align*}
Thus we have
\begin{align*}
&\left| \langle \Psi(0), P^i_+(0; \lambda) \Phi^c_{i,+}(0, X_i; \lambda) P^i_+(X_i, \lambda)^{-1} a_i^c \rangle \right| \leq C |a_i^c| \\
&\qquad\leq C |\lambda|(e^{-\alpha X^*} + |\lambda|) \left( |c| + (|\lambda| + e^{-\alpha X^*})^2  |d| \right)
\end{align*}
The other term is similar.

\item For the terms involving $b$, the terms $P_-(0; 0) b_i^-$ and $P_+(0, 0)b_i^+$ are eliminated outright when we take the inner product with $\Psi(0)$. For the other terms, we use the estimate for $B_1$ from Lemma \ref{Zinv2}.
\begin{align*}
\left| \langle \Psi(0), (P^i_+(0; \lambda) - P^i_+(0; 0))b_i^+ + P^i_+(0; \lambda) (P^s(\lambda) - P^s(0)) b_i^+ \rangle \right| \leq C |\lambda| \left( e^{-\alpha X^*}|c| + (|\lambda| + e^{-\alpha X^*})^2 |d| \right)
\end{align*}
The $b_i^-$ term is similar.

\item Finally, we look at the integral terms. For the center integral terms involving $\tilde{H}_i^\pm$, as in \cref{jumpcenteradj},
\begin{align*}
\langle \Psi(0), &P^i_-(0; \lambda) \lambda^2 d_i \int_{-X_{i-1}}^0 \Phi^c_{i,-}(0, y; \lambda) P^i_-(y; \lambda)^{-1} \tilde{H}_i^-(y) dy \rangle \\
&= \lambda^2 d_i \int_{-X_{i-1}}^0 \langle \tilde{\Phi}^*_-(y, -X_{i-1}; 0) [P^c(0)^*] \tilde{\Phi}^*_-(-X_{i-1}, 0; 0) \Psi(0),
 H(y) \rangle dy + \mathcal{O}(|\lambda|^3 |d|) \\
&= \lambda^2 d_i \int_{-X_{i-1}}^0 \langle \tilde{\Phi}^*_-(y, -X_{i-1}; 0)^* P^{c,*}(0) \Psi(-X_{i-1}),
 H(y) \rangle dy + \mathcal{O}(|\lambda|^3 |d|) \\
 &= \mathcal{O}(|\lambda|^2 (|\lambda| + e^{-\alpha X_*}) |d|)
\end{align*}
where $[P^c(0)^*] = P^{c,*}(0)$ by \cref{lemma:Afacts} and $P^{c,*}(0) \Psi(-X_{i-1}) = \mathcal{O}(e^{-2 \alpha X_{i-1}})$. The other integral term is similar. For the center integral terms involving $G_i^\pm$, we similarly have
\begin{align*}
\langle \Psi(0), &P^i_-(0; \lambda) \int_{-X_{i-1}}^0 \Phi^c_{i,-}(0, y; \lambda) P^i_-(y; \lambda)^{-1} c_{i-1} e^{\nu(\lambda)X_{i-1}} G_i^-(y) V^-(y; \lambda) dy \rangle \\
&= c_{i-1} e^{\nu(\lambda)X_{i-1}}\int_{-\infty}^0 \langle \tilde{\Phi}^*_-(y, -X_{i-1}; 0) P^{c,*}(0) \Psi(-X_{i-1}), G_i^-(y) V^-(y; \lambda)  \rangle dy + \mathcal{O}(|\lambda| e^{-\alpha X^*} |c|) \\
&= \mathcal{O}(e^{-\alpha X^*}(|\lambda| + e^{-\alpha X^*}) |c|)
\end{align*}
The bound on the non-center integral involving $G_i^\pm$ is stronger than the bound on the corresponding center integral, and is thus subsumed by this bound,
\end{enumerate}

Putting this all together, we have the jump expressions
\begin{align*}
\xi_i = \langle \Psi&(X_i), Q'(-X_i) \rangle (d_{i+1} - d_i ) + \langle \Psi(-X_{i-1}), Q'(X_{i-1}) \rangle (d_i - d_{i-1} ) \\
&-\frac{1}{2}\lambda M^c\left( e^{-\nu(\lambda)X_i}c_i + e^{\nu(\lambda)X_i}c_{i-1}\right)
- \lambda^2 d_i M + R_i(\lambda)(c, d)
\end{align*}
where $M$ is the higher order Melnikov integral
\[
M = \int_{-\infty}^\infty \langle \Psi(y), H(y) \rangle dy,
\]
$M^c$ is the center Melnikov integral defined in \cref{lemma:VderivIPs}, and the remainder term bound
\begin{equation}\label{noncenterR}
|R(\lambda)(c, d)| \leq C \left( (e^{-\alpha X^*} + |\lambda|)^2 |c| + (e^{-\alpha X^*} + |\lambda|)^3 |d| \right)
\end{equation}

As in Lemma \ref{jumpcenteradj}, we will write these jump expressions in matrix form. The leading order terms involving $c$ are given by the matrix $-\frac{1}{2}\lambda M^c K_1(\lambda)c$, where $K_1(\lambda)$ is the periodic, bi-diagonal matrix
\begin{align*}
K_1(\lambda) =  
\begin{pmatrix}
e^{-\nu(\lambda)X_1} & & & & & e^{\nu(\lambda)X_0} \\
e^{\nu(\lambda)X_1} & e^{-\nu(\lambda)X_2} \\
& e^{\nu(\lambda)X_2} & e^{-\nu(\lambda)X_3} \\
 & & \ddots & &&   \\
& & & & e^{\nu(\lambda)X_{n-1}} & e^{\nu(\lambda)X_0}
\end{pmatrix}
\end{align*}
We note that $K_1(\lambda)$ is the same matrix as $K(\lambda)$ in the previous lemma with all terms positive.

For the terms involving $d$. Let
\[
a_i = \langle \Psi(X_i), Q'(-X_i) \rangle 
\]
By reversibility, $Q(-x) = R Q(x)$ implies $Q'(-x) = -R Q'(x)$. From Lemma \ref{varadjsolutions}, $\Psi(x) = R \Psi(-x)$. Thus, since $R^2 = I$ and $R$ is self-adjoint, we have
\begin{align*}
\langle \Psi(-X_i), Q'(X_i) \rangle &= \langle \Psi(-X_i), R^2 Q'(X_i) \rangle \\
&= -\langle R \Psi(-X_i), Q'(-X_i) \rangle \\
&= -\langle \Psi(X_i), Q'(-X_i) \rangle \\
&= -a_i
\end{align*}
Thus the leading order terms involving $d$ are given in matrix form by $(A - \lambda^2 M I + D_2)d$, where the $A$ is given by
\begin{align*}
A &= \begin{pmatrix}
-a_{n-1} - a_0 & a_0 & & & \dots & a_{n-1}\\
a_0 & -a_0 - a_1 &  a_1 \\
& a_1 & -a_1 - a_2 &  a_2 \\
& & \vdots & & \vdots \\
a_{n-1} & & & & a_{n-2} & -a_{n-2} - a_{n-1} \\
\end{pmatrix}
\end{align*}
Let $C_2$ and $D_2$ be the matrices we get from the remainder terms involving $c$ and $d$. Combining everything above gives us the matrix form \cref{Psimatrix}. Since $e^{-\alpha X^*} = C r^{1/2}$, $C_2$ and $D_2$ have the bounds in \cref{adjjumprem}.
\end{proof}
\end{lemma}

\section{Proof of Theorem \ref{blockmatrixtheorem}}

Theorem \ref{blockmatrixtheorem} combines the jump matrix formulas from Lemma \ref{jumpcenteradj} and Lemma \ref{jumpadj} into a single block matrix. Using the definitions of $H(y)$ and $B$ and equation \cref{psicomponents} for $\Psi(y)$, we can compute the higher order Melnikov integral.
\begin{align*}
M = \int_{-\infty}^\infty \langle \Psi(y), H(y) \rangle dy = \int_{-\infty}^\infty q(y) \partial_c q(y) dy
\end{align*}

\section{Characterization of matrix $A$}

Before we conclude this section, we will prove some results based on \cref{blockmatrixtheorem}. In this section, we will characterize the matrix $A$ in the lower left block of the block matrix \cref{blockeq}. 

\begin{lemma}\label{lemma:ajparam}
For $r \leq r_*$, the terms $a_j$ in the block matrix equation \cref{blockeq} have the form
\[
a_j = r \tilde{a}^j(r),
\]
where
\begin{equation}\label{ajparam}
\tilde{a}_j(r) = -p_0 e^{\alpha \phi/\beta_0} b_j \left( \beta \cos\left(-\rho \log b_j \right) - \alpha \sin \left(-\rho \log b_j \right) \right) + \mathcal{O}(r^{\gamma/2\alpha}),
\end{equation}
$p_0 > 0$, and
\begin{equation}\label{bj2}
b_j = e^{-2 \alpha (X_j - X^*)}
\end{equation}

\begin{proof}
Using \cite[Lemma 6.1]{Sandstede1998} and making the same modifications as we did in Lemma \ref{IPform},
\begin{align*}\label{IPpsiQprime}
\langle \Psi(-x), Q'(x) \rangle
&= p_0 e^{-2 \alpha x}\left( \beta_0 \cos(2 \beta_0 x + \phi) - \alpha \sin(2 \beta_0 x + \phi)\right) + \mathcal{O}(e^{-(2 \alpha + \gamma) x}
\end{align*}
where $p_0 > 0$ and $\gamma$ are the same as in Lemma \ref{IPform}. From the proof of Lemma \ref{jumpadj}, $\langle \Psi(X_j), Q'(-X_j) \rangle = - \langle \Psi(-X_j), Q'(X_j) \rangle$. Using equation \cref{Xjscale} for $X_j$, we have
\begin{align*}
a_j(r) &= \langle \Psi(X_j), Q'(-X_j) \rangle = -\Psi(-X_j), Q'(X_j) \rangle \\
&= -s_0 e^{-2 \alpha X_j}\left( \beta_0 \cos(2 \beta_0 X_j + \phi) - \alpha \sin(2 \beta_0 X_j + \phi)\right) + \mathcal{O}(e^{-(2 \alpha + \gamma_0) X_j}) \\
&= -s_0 e^{\alpha \phi/\beta_0} r b_j \left( \beta_0 \cos\left( -\frac{\beta_0}{\alpha} \log(b_j r) \right) - \alpha \sin \left( -\frac{\beta_0}{\alpha} \log(b_j r) \right) \right) + \mathcal{O}(r^{1+\gamma/2\alpha} b_j^{1 + \gamma/2\alpha}) \\
&= -s_0 e^{\alpha \phi/\beta_0} r b_j \left( \beta_0 \cos\left( -\rho \log(b_j r) \right) - \alpha \sin \left( -\rho \log(b_j r) \right) \right) + \mathcal{O}(r^{1+\gamma/2\alpha})
\end{align*}
since $b_j \in (0, 1]$. Since $r \in \mathcal{R}$, $r = \exp\left(-\frac{2 m \pi}{\rho}\right)$ for some nonnegative integer $m$, this becomes 
\begin{align*}
a_j(r) &= -s_0 e^{\alpha \phi/\beta_0} r b_j \left( \beta_0 \cos\left( 2 m \pi -\rho \log b_j \right) - \alpha \sin \left( 2 m \pi -\rho \log b_j \right) \right) + \mathcal{O}(r^{1+\gamma/2\alpha}) \\
&= -s_0 e^{\alpha \phi/\beta_0} r b_j \left( \beta_0 \cos\left(-\rho \log b_j \right) - \alpha \sin \left(-\rho \log b_j \right) \right) + \mathcal{O}(r^{1+\gamma/2\alpha})
\end{align*}
The result follows from letting $a_j(r) = r \tilde{a}_j(r)$.
\end{proof}
\end{lemma}

We can now characterize the matrix $A$.

\begin{lemma}\label{lemma:tildeA}
For $r \leq r_*$, the matrix $A$ in \cref{blockeq} has the form
\begin{equation}\label{deftildeA}
A = r \tilde{A}(r)
\end{equation}
where $\tilde{A}(r) = \tilde{A}(r; m_0, \dots, m_{n-1}, \theta)$ is symmetric and continuous in $r$. $\tilde{A}(r)$ has an eigenvalue of 0 corresponding to eigenvector $(1, 1, \dots, 1)^T$. The remaining eigenvalues $\ell_1(r), \dots, \ell_{n-1}(r) \}$ of $\tilde{A}(r)$ are real and are continuous in $r$.
\begin{proof}
By \cref{lemma:ajparam}, we can scale out $r$ from each of the terms $a_j = r \tilde{a}_j(r)$ in \cref{blockeq} to obtain \cref{deftildeA}. Since all of the $\tilde{a}_j(r)$ are continuous in $r$, $\tilde{A}$ is as well. Since $A$ is symmetric, $\tilde{A}(r)$ is also symmetric, thus its eigenvalues are real. The kernel eigenvector can be verified directly since all rows of $\tilde{A}$ sum to 0.
\end{proof}
\end{lemma}

\section{Center eigenfunction}

Recall that when $\lambda = 0$, equation \cref{PDEeigsystemper2} has a solution $\partial_x Q_n(x)$. 
In this section, we will show that under certain conditions, there is another solution to equation \cref{PDEeigsystemper2} when $\lambda = 0$.

\begin{lemma}\label{lemma:centereigenfn1}
If the kernel of the operator $\calL(q_n)$ on $H^{2m}_{\text{per}}[-X,X]$ is simple, there exists a function $V_n^c(x)$ which satisfies
\begin{align*}
[V_n^c]'(x) &= A(Q_n(x))V_n^c(x) \\
V_n^c(-X) &= V_n^c(X)
\end{align*}
\begin{proof}
Consider the equation
\begin{equation}\label{Lqn1}
\calL(q_n) v = 1
\end{equation}
posed on $H^{2m}_{\text{per}}[-X,X]$. Since both $q_n$ and the constant function $1$ are in $H^{2m}_{\text{per}}[-X,X]$, this is well-defined. The operator $\calL(q_n)$ is self-adjoint, and $\partial_x q_n \in \ker \calL(q_n)$. Integrating by parts and noting that the boundary term cancels due to the periodic boundary conditions,
\[
\langle \partial_x q_n(x), 1 \rangle_{H^{2m}_{\text{per}}[-X,X]} = 0
\]
Assuming that the kernel of $\calL(q_n)$ is simple, it follows from follows from the Fredholm alternative that \cref{Lqn1} has a solution $v(x) \in {H^{2m}_{\text{per}}[-X,X]}$. Let
\[
V_n^c = \left( v(x), \partial_x v(x), \dots, \partial_x^{2m-1}(x), 1 \right)
\]
Then $V_n^c(-X) = V_n^c(X)$, and from the definition of $A(Q_n(x))$, $[V_n^c]'(x) = A(Q_n(x))V_n^c(x)$.
\end{proof}
\end{lemma}

For the conclusion of \cref{lemma:centereigenfn1} to hold, we need a condition for when $\calL{q_n}$ has a simple kernel. Using a spatial dynamics formulation, the eigenvalue problem $\calL{q_n}v = \lambda v$ is equivalent to the first order system of ODEs 
\begin{equation}\label{Lsystem1}
\begin{aligned}
V'(x) &= DF(Q_n(x))V(x) + \lambda B V(x) \\
V(-X) &= V(X)
\end{aligned}
\end{equation}
where $V(x) \in C^0(\R, R^{2m})$. When $\lambda = 0$, $\partial_x Q(x)$ is a solution. In the next lemma, we give a condition for which this is the only solution.

\begin{lemma}\label{Lsystemeigs}
If the eigenvalues of $\tilde{A}(0)$ are distinct, then for sufficiently small $r$, the only solution to \cref{Lsystem1} when $\lambda = 0$ is $\partial_x Q(x)$.
\begin{proof}
Since the matrix $DF(0)$ is hyperbolic, solutions to \cref{Lsystem1} can be found using the method in \cite{Sandstede1998} adapted to periodic boundary conditions. Briefly, this works as follows. The setup is exactly the same as in \cite{Sandstede1998}, except periodic boundary conditions require one more matching condition at the tails of the pulses to ``close the loop''. Following the proof of \cite[Theorem 2]{Sandstede1998}, an eigenfunction $V(x)$ exists for sufficiently small $\lambda$ if and only if the $n$ jump conditions
\begin{align*}
\xi_i = \langle \Psi(X_i), &\partial_x Q(-X_i) \rangle (d_{i+1} - d_i) + \Psi(-X_{i-1}), \partial_x Q(X_{i-1}) \rangle (d_i - d_{i-1}) \\
&- d_i \int_{-\infty}^\infty \langle \Psi(y) B \partial_x Q(y) \rangle dy + R(\lambda)_i d = 0
\end{align*}
are satisfied, where $\tilde{\Psi}(x) = \nabla H(Q(x))$ is the unique bounded solution to the adjoint variational equation \cref{adjvareq1} and the remainder term has bound
\[
|R(\lambda)d| \leq C \left( e^{-3 \alpha X^*} + |\lambda|(e^{-\alpha X^*} + |\lambda| ) \right)
\]
This is analogous to \cite[(3.56)]{Sandstede1998}. By Remark \ref{remark:psinotation}, the inner product $\langle \Psi(x), \partial_x Q(y) \rangle$ are the same for the existence and the stability problem, therefore the jump conditions can be written in matrix form as in \cite[Theorem 2]{Sandstede1998} as
\begin{equation}\label{Ljumps}
E(\lambda) = \det S(\lambda) = \det( A - M_1 \lambda I + R(\lambda)) = 0
\end{equation}
where $A$ the same matrix as in \cref{blockmatrixtheorem} and
\[
M_1 = 
\int_{-\infty}^\infty \langle \tilde{\Psi}(y) B \partial_x Q(y) \rangle dy =  
\int_{-\infty}^\infty [\partial_y q(y)]^2 dy > 0
\]
By \cref{lemma:tildeA}, $A = r \tilde{A}(r)$, where $\tilde{A}(r)$ is continuous in $r$ and has an eigenvalue at 0 for all $r$. If the eigenvalues of $\tilde{A}(0)$ are distinct, $\tilde{A}(0)$ has a simple eigenvalue at 0. Following the proof of \cite[Theorem 3]{Sandstede1998}, for sufficiently small $r$, equation \cref{Ljumps} has a simple zero at 0. Since this zero must correspond to $\partial_x Q_n(x)$, the result follows.
\end{proof}
\end{lemma}

We combine the two previous lemmas to get the following result.

\begin{lemma}\label{lemma:centereigenfn}
If the eigenvalues of $\tilde{A}(0)$ are distinct, then for sufficiently small $r$ there exists a function $V_n^c(x)$ which satisfies \cref{PDEeigsystemper3} for $\lambda = 0$.
\end{lemma}

\iffulldocument\else
	\bibliographystyle{amsalpha}
	\bibliography{thesis.bib}
\fi

\end{document}